lean/privacy/no_replay.lean
@@ -22,11 +22,11 @@ theorem no_replay
   case OpenChannel inp =>
     let info := open_channel_info crypto inp rm success
     have ⟨channel_imp⟩ := ChannelImplies.from_action h
-    exact channel_imp.channel_hashes info.channel_didnt_exist
+    exact channel_imp.channel_markers info.channel_didnt_exist
   case OpenSubchannel inp =>
     let info := open_subchannel_info crypto inp rm success
     have ⟨subchannel_imp⟩ := SubchannelImplies.from_action h
-    exact subchannel_imp.subchannel_hash info.old_hash_was_zero
+    exact subchannel_imp.subchannel_marker info.old_hash_was_zero
   case CreateNote inp =>
     let info := create_note_info crypto inp rm success
     have ⟨note_imp⟩ := NoteImplies.from_action h
