lean/privacy/notes/note_implies.lean
@@ -91,7 +91,7 @@ theorem NoteImplies.from_action
   cases h
   case head =>
     let info := create_note_info crypto inp rm success
-    have ⟨addralice, ⟨subchannel_imp⟩⟩ := SubchannelImplies.from_subchannel_hash_exists info.subchannel_exists
+    have ⟨addralice, ⟨subchannel_imp⟩⟩ := SubchannelImplies.from_subchannel_marker_exists info.subchannel_exists
     have h_addralice: inp.addralice = addralice := by
       simp [subchannel_imp.channel.same_c (Eq.symm subchannel_imp.h_c)]
 
